\section{Fibonnacci Numbers}

\[ F_{n} = F_{n-1} + F_{n-2} \mbox{ For }\]

%-------------------------------------%


{Proof by Induction}

Let the summation $s_n$ be defined as follows:
\[s_n = 1 + 3 + 5 + \ldots + (2n − 1) \] for $n \in \mathbb{Z}^{+}$.

Use the method of induction to prove that $s_n = n^2$ for all $n \geq 1$.


%------------------------------------------- %

%------------------------------------%

{Fibonnacci Numbers}

\[ F_{n} = F_{n-1} + F_{n-2} \mbox{ For }\]

%-------------------------------------%


{Proof by Induction}

Let the summation $s_n$ be defined as follows:
\[s_n = 1 + 3 + 5 + \ldots + (2n − 1) \] for $n \in \mathbb{Z}^{+}$.

Use the method of induction to prove that $s_n = n^2$ for all $n \geq 1$.


%------------------------------------------- %

\end{document}
